\begin{equation}
    \hat{\boldsymbol{\Gamma}}_{\mathcal{N}_{\mathrm{adj}_{2}}}
    =
    A_{0}^{-1} B_{0} A_{0}^{-1}
\end{equation}

\begin{equation}
    A_{0}
    =
    -
    \sum_{i = 1}^{n}
    \frac{
      \partial
      \ell_{i}
    }{
      \partial
      \hat{\boldsymbol{\sigma}}
      \partial
      \hat{\boldsymbol{\sigma}}^{\prime}
    }
\end{equation}

\begin{equation}
  B_{0}
  =
  \sum_{i = 1}^{n} 
  \left(
  \frac{
  \partial 
  \ell_{i}
  }{
  \partial
  \hat{\boldsymbol{\sigma}}
  }
  \right) 
  \times
  \left(
  \frac{
  \partial 
  \ell_{i}
  }{
  \partial 
  \hat{\boldsymbol{\sigma}}
  }
  \right)^{\prime}
\end{equation}